project/Elementary_CA_Base.thy
@@ -17,16 +17,40 @@ fun sum_nb :: "neighbourhood \<Rightarrow> nat" where
 "sum_nb (Nb a b c) = count_list [a, b, c] One"
 
 
+lemma flip_nb_cancel [simp]: "flip_nb (flip_nb nb) = nb"
+apply(induction nb)
+apply(auto)
+done
+
+lemma sum_nb_bound: "sum_nb nb \<le> 3"
+apply(induction nb)
+apply(auto)
+done
+
+
 subsection \<open>Basic Rule Properties\<close>
 
 fun mirror :: "rule \<Rightarrow> rule" where
 "mirror r (Nb a b c)= r (Nb c b a)"
 
+lemma [simp]: "(mirror (mirror r)) a = r a"
+apply(induction a)
+apply(auto)
+done
+
+
 definition amphichiral :: "rule \<Rightarrow> bool" where
-"amphichiral r \<equiv> r = (mirror r)"
+"amphichiral r \<equiv> (\<forall> c. r c = (mirror r) c)"
 
 fun complement :: "rule \<Rightarrow> rule" where
 "complement r nb = flip (r (flip_nb nb))"
+
+
+lemma [simp]: "complement (complement r) a = r a"
+apply(induction a)
+apply auto
+done
+
 
 definition totalistic :: "rule \<Rightarrow> bool" where
 "totalistic r \<equiv> (\<forall> nb1 nb2. sum_nb nb1 = sum_nb nb2 \<longrightarrow> (r nb1) = (r nb2))"
@@ -37,6 +61,19 @@ subsection \<open>Concrete rule examples\<close>
 definition null_rule :: rule where
 "null_rule _ = Zero"
 
+fun r4 :: rule where
+"r4  (Nb One  One  One)  = Zero" |
+"r4  (Nb One  One  Zero) = Zero" |
+"r4  (Nb One  Zero One)  = Zero" |
+"r4  (Nb One  Zero Zero) = Zero" |
+"r4  (Nb Zero One  One)  = Zero" |
+"r4  (Nb Zero One  Zero) = One"  |
+"r4  (Nb Zero Zero One)  = Zero" |
+"r4  (Nb Zero Zero Zero) = Zero"
+
+
+subsection \<open>Rule 110\<close>
+
 fun r110 :: rule where
 "r110  (Nb One  One  One)  = Zero" |
 "r110  (Nb One  One  Zero) = One"  |
@@ -46,5 +83,16 @@ fun r110 :: rule where
 "r110  (Nb Zero One  Zero) = One"  |
 "r110  (Nb Zero Zero One)  = One"  |
 "r110  (Nb Zero Zero Zero) = Zero"
+
+lemma "\<not>amphichiral r110"
+apply auto
+by (metis amphichiral_def cell.distinct(1) mirror.simps r110.simps(4) r110.simps(7))
+
+lemma "\<not>totalistic r110"
+apply auto
+apply(simp add: totalistic_def)
+apply(rule allE)
+apply auto
+by (metis cell.simps(2) count_list.simps(2) r110.simps(4) r110.simps(6) sum_nb.simps)
 
 end
