project/Infinite_Elementary_CA.thy
@@ -14,35 +14,46 @@ fun update_state :: "CA \<Rightarrow> state" where
 fun update_CA :: "CA \<Rightarrow> CA" where
 "update_CA (CA s r) = CA (update_state (CA s r)) r"
 
-fun run_t_steps :: "CA \<Rightarrow> nat \<Rightarrow> CA" where
-"run_t_steps ca n = apply_t_times update_CA ca n"
+fun run :: "CA \<Rightarrow> nat \<Rightarrow> CA" where
+"run ca n = apply_t_times update_CA ca n"
 
-
-subsection \<open>Example CAs\<close>
-
-definition state1 :: state where
-"state1 s \<equiv> (if s = 0 then One else Zero)"
-
-definition rule110 :: CA where
-"rule110 \<equiv> CA state1 r110"
-
-value "State (run_t_steps rule110 5) (-3)"
-
+lemma [simp]: "run ca 0 = ca"
+apply auto
+done
 
 subsection \<open>Properties\<close>
 
 definition stable :: "CA \<Rightarrow> bool" where
-"stable ca \<equiv> State (update_CA ca) = State ca"
+"stable ca \<equiv> (\<forall> c. State (update_CA ca) c = (State ca) c)"
 
 (*This def works only because we have binary cells*)
 definition uniform :: "state \<Rightarrow> bool" where
 "uniform s \<equiv> \<not> (surj s)"
 
 definition yields :: "CA \<Rightarrow> state \<Rightarrow> bool" (infixr \<open>yields\<close>  65) where
-"A yields s \<equiv> (\<exists> n. State (run_t_steps A n) = s \<and> n > 0)"
+"A yields s \<equiv> (\<exists> n. State (run A n) = s \<and> n > 0)"
+
+theorem "n>0 \<Longrightarrow> ca yields State (run ca n)"
+  apply(simp add: yields_def)
+  apply(rule exI)
+  apply(rule conjI)
+  apply(auto)
+done
 
 definition loops :: "CA \<Rightarrow> bool" where
 "loops ca \<equiv> ca yields State ca"
+
+lemma "loops ca \<Longrightarrow> (\<exists> n. State (run ca n) = State ca)"
+apply auto
+apply(simp add: loops_def)
+apply(simp add: yields_def)
+apply(auto)
+done
+
+theorem cycle: "loops ca \<Longrightarrow> (\<exists> m n. (\<forall> k. State (run ca (n + (k*m))) = State ca))"
+apply auto
+by (metis add_cancel_right_right apply_t_times.simps(1) mult_0 semiring_normalization_rules(7))
+
 
 fun reversible :: "CA \<Rightarrow> bool" where
 "reversible (CA _ r) = (\<forall>s. (\<exists>!s0. State (update_CA (CA s0 r)) = s))"
@@ -51,7 +62,11 @@ fun garden_of_eden :: "CA \<Rightarrow> bool" where
 "garden_of_eden (CA s r) = (\<not>(\<exists> s0. State (update_CA (CA s0 r)) = s))"
 
 lemma "garden_of_eden ca \<Longrightarrow> \<not>reversible ca"
-  by (metis garden_of_eden.elims(2) reversible.simps)
+by (metis garden_of_eden.elims(2) reversible.simps)
+
+(* TODO see if a definition can be made work for infinite compared to finite *)
+(*definition orphan :: "state \<Rightarrow> rule \<Rightarrow> bool" where
+"orphan s0 r = (\<forall> sl sr. garden_of_eden (CA (sl@s0@sr) r))"*)
 
 
 definition class1 :: "rule \<Rightarrow> bool" where
@@ -63,14 +78,28 @@ definition class2 :: "rule \<Rightarrow> bool" where
 lemma "class1 ca \<Longrightarrow> class2 ca"
   using class1_def class2_def loops_def by auto
 
-
-subsection \<open>Concrete examples\<close>
+  
+subsection \<open>Example CAs\<close>
 
 definition zero_state :: state where
 "zero_state _ \<equiv> Zero"
 
+definition state1 :: state where
+"state1 s \<equiv> (if s = 0 then One else Zero)"
+
+definition rule110 :: CA where
+"rule110 \<equiv> CA state1 r110"
+
+value "State (run rule110 5) (-3)"
+
+lemma "stable (CA state1 r4)"
+apply(simp add: stable_def)
+apply auto
+by (simp add: state1_def)
+
+(*TODO make lem more interesting by showing a late stage of some rule is uniform*)
 lemma "uniform zero_state"
   apply(simp add: zero_state_def uniform_def)
   apply(auto)
-  done
+done
 end
